<?xml version="1.0"?>
<rdf:RDF xmlns="http://ns.peterkrantz.se/flashcards/2018#"
     xml:base="http://ns.peterkrantz.se/flashcards/2018"
     xmlns:dc="http://purl.org/dc/elements/1.1/"
     xmlns:dct="http://purl.org/dc/terms/"
     xmlns:fco="http://ns.peterkrantz.se/flashcards/2018#"
     xmlns:owl="http://www.w3.org/2002/07/owl#"
     xmlns:rdf="http://www.w3.org/1999/02/22-rdf-syntax-ns#"
     xmlns:xml="http://www.w3.org/XML/1998/namespace"
     xmlns:xsd="http://www.w3.org/2001/XMLSchema#"
     xmlns:rdfs="http://www.w3.org/2000/01/rdf-schema#"
     xmlns:vann="http://purl.org/vocab/vann/"
     xmlns:schema="http://schema.org/">
    <owl:Ontology rdf:about="http://ns.peterkrantz.se/flashcards/2018#">
        <dc:creator>Peter Krantz</dc:creator>
        <dct:abstract xml:lang="en">This document also contains examples of serialization in XML and JSON.</dct:abstract>
        <dct:license rdf:resource="http://creativecommons.org/licenses/by/4.0/"/>
        <rdfs:comment xml:lang="en">This vocabulary describes flash cards. A flash card contains information such as words, numbers or images. Flash cards are used by students in classroom drills or in private study to improve memorization. A card contains the information being studied and is, optionally, divided into a question and a related answer. Multiple related cards can be grouped in a stack.</rdfs:comment>
        <rdfs:label xml:lang="en">Flash card ontology</rdfs:label>
    </owl:Ontology>
    


    <!-- 
    ///////////////////////////////////////////////////////////////////////////////////////
    //
    // Annotation properties
    //
    ///////////////////////////////////////////////////////////////////////////////////////
     -->

    


    <!-- http://purl.org/dc/terms/hasPart -->

    <owl:AnnotationProperty rdf:about="http://purl.org/dc/terms/hasPart"/>
    


    <!-- http://purl.org/dc/terms/isPartOf -->

    <owl:AnnotationProperty rdf:about="http://purl.org/dc/terms/isPartOf"/>
    


    <!-- 
    ///////////////////////////////////////////////////////////////////////////////////////
    //
    // Data properties
    //
    ///////////////////////////////////////////////////////////////////////////////////////
     -->

    


    <!-- http://ns.peterkrantz.se/flashcards/2018#mediaItem -->

    <owl:DatatypeProperty rdf:about="http://ns.peterkrantz.se/flashcards/2018#mediaItem">
        <rdfs:subPropertyOf rdf:resource="http://www.w3.org/2002/07/owl#topDataProperty"/>
        <rdfs:domain rdf:resource="http://ns.peterkrantz.se/flashcards/2018#Card"/>
        <rdfs:comment xml:lang="en">Media item data for a audio, an image or other types of media.</rdfs:comment>
        <rdfs:label xml:lang="en">media</rdfs:label>
    </owl:DatatypeProperty>
    


    <!-- http://ns.peterkrantz.se/flashcards/2018#relatedWork -->

    <owl:DatatypeProperty rdf:about="http://ns.peterkrantz.se/flashcards/2018#relatedWork">
        <rdfs:subPropertyOf rdf:resource="http://www.w3.org/2002/07/owl#topDataProperty"/>
        <rdfs:domain rdf:resource="http://ns.peterkrantz.se/flashcards/2018#Stack"/>
        <rdfs:comment xml:lang="en">A related creative work as e.g. a book, a book chapter, a movie or song. This property can be used to connect a stack of cards to a vocabulary from a chapter in a language textbook.</rdfs:comment>
        <rdfs:label xml:lang="en">related work</rdfs:label>
    </owl:DatatypeProperty>
    


    <!-- http://ns.peterkrantz.se/flashcards/2018#sortOrder -->

    <owl:DatatypeProperty rdf:about="http://ns.peterkrantz.se/flashcards/2018#sortOrder">
        <rdfs:domain rdf:resource="http://ns.peterkrantz.se/flashcards/2018#Card"/>
        <rdfs:range rdf:resource="http://www.w3.org/2001/XMLSchema#positiveInteger"/>
        <rdfs:comment xml:lang="en">The initial card sort order expressed as an integer value. The sort order should be used as a suggestion, e.g. when no other sort order exists, and may be ignored by users and tools.</rdfs:comment>
        <rdfs:label xml:lang="en">sort order</rdfs:label>
    </owl:DatatypeProperty>
    


    <!-- http://ns.peterkrantz.se/flashcards/2018#text -->

    <owl:DatatypeProperty rdf:about="http://ns.peterkrantz.se/flashcards/2018#text">
        <rdfs:domain rdf:resource="http://ns.peterkrantz.se/flashcards/2018#Card"/>
        <rdfs:comment xml:lang="en">Text content for this object.</rdfs:comment>
        <rdfs:label xml:lang="en">text</rdfs:label>
    </owl:DatatypeProperty>
    


    <!-- 
    ///////////////////////////////////////////////////////////////////////////////////////
    //
    // Classes
    //
    ///////////////////////////////////////////////////////////////////////////////////////
     -->

    


    <!-- http://ns.peterkrantz.se/flashcards/2018#Answer -->

    <owl:Class rdf:about="http://ns.peterkrantz.se/flashcards/2018#Answer">
        <dct:isPartOf rdf:resource="http://ns.peterkrantz.se/flashcards/2018#Card"/>
        <rdfs:comment xml:lang="en">An answer to a related test.</rdfs:comment>
        <rdfs:label xml:lang="en">Answer</rdfs:label>
    </owl:Class>
    


    <!-- http://ns.peterkrantz.se/flashcards/2018#Card -->

    <owl:Class rdf:about="http://ns.peterkrantz.se/flashcards/2018#Card">
        <dct:isPartOf rdf:resource="http://ns.peterkrantz.se/flashcards/2018#Stack"/>
        <rdfs:comment xml:lang="en">A physical or virtual card bearing information such as words, images or numbers, on either or both sides. Used in classroom drills or in private study. The card has an associated test and an answer.</rdfs:comment>
        <rdfs:label xml:lang="en">Card</rdfs:label>
    </owl:Class>
    


    <!-- http://ns.peterkrantz.se/flashcards/2018#Stack -->

    <owl:Class rdf:about="http://ns.peterkrantz.se/flashcards/2018#Stack">
        <dct:hasPart rdf:resource="http://ns.peterkrantz.se/flashcards/2018#Card"/>
        <rdfs:comment xml:lang="en">A stack represents a collection of cards and is typically used to group cards belonging to a topic being studied. E.g. a collection of cards containing vocabulary for a chapter in a language textbook.</rdfs:comment>
        <rdfs:label xml:lang="en">Stack</rdfs:label>
    </owl:Class>
    


    <!-- http://ns.peterkrantz.se/flashcards/2018#Test -->

    <owl:Class rdf:about="http://ns.peterkrantz.se/flashcards/2018#Test">
        <dct:isPartOf rdf:resource="http://ns.peterkrantz.se/flashcards/2018#Card"/>
        <rdfs:comment xml:lang="en">The information the user is trying to memorize. Representing the front side of a physical card.</rdfs:comment>
        <rdfs:label xml:lang="en">Test</rdfs:label>
    </owl:Class>
    


    <!-- 
    ///////////////////////////////////////////////////////////////////////////////////////
    //
    // General axioms
    //
    ///////////////////////////////////////////////////////////////////////////////////////
     -->

    <rdf:Description>
        <rdf:type rdf:resource="http://www.w3.org/2002/07/owl#AllDisjointClasses"/>
        <owl:members rdf:parseType="Collection">
            <rdf:Description rdf:about="http://ns.peterkrantz.se/flashcards/2018#Answer"/>
            <rdf:Description rdf:about="http://ns.peterkrantz.se/flashcards/2018#Card"/>
            <rdf:Description rdf:about="http://ns.peterkrantz.se/flashcards/2018#Stack"/>
            <rdf:Description rdf:about="http://ns.peterkrantz.se/flashcards/2018#Test"/>
        </owl:members>
    </rdf:Description>
</rdf:RDF>



<!-- Generated by the OWL API (version 4.5.6.2018-09-06T00:27:41Z) https://github.com/owlcs/owlapi -->

