@prefix : <http://ns.peterkrantz.se/flashcards/2018#> .
@prefix owl: <http://www.w3.org/2002/07/owl#> .
@prefix rdf: <http://www.w3.org/1999/02/22-rdf-syntax-ns#> .
@prefix xml: <http://www.w3.org/XML/1998/namespace> .
@prefix xsd: <http://www.w3.org/2001/XMLSchema#> .
@prefix rdfs: <http://www.w3.org/2000/01/rdf-schema#> .
@base <http://ns.peterkrantz.se/flashcards/2018#> .

<http://ns.peterkrantz.se/flashcards/2018#> rdf:type owl:Ontology ;
                                             <http://purl.org/dc/elements/1.1/creator> "Peter Krantz" ;
                                             <http://purl.org/dc/terms/abstract> "This document also contains examples of serialization in XML and JSON."@en ;
                                             <http://purl.org/dc/terms/license> <http://creativecommons.org/licenses/by/4.0/> ;
                                             rdfs:comment "This vocabulary describes flash cards. A flash card contains information such as words, numbers or images. Flash cards are used by students in classroom drills or in private study to improve memorization. A card contains the information being memorized and is divided into a question and a related answer. Multiple related cards can be grouped in a stack."@en ;
                                             rdfs:label "Flash card ontology"@en .

#################################################################
#    Annotation properties
#################################################################

###  http://purl.org/dc/terms/hasPart
<http://purl.org/dc/terms/hasPart> rdf:type owl:AnnotationProperty .


###  http://purl.org/dc/terms/isPartOf
<http://purl.org/dc/terms/isPartOf> rdf:type owl:AnnotationProperty .


#################################################################
#    Data properties
#################################################################

###  http://ns.peterkrantz.se/flashcards/2018#mediaItem
:mediaItem rdf:type owl:DatatypeProperty ;
           rdfs:subPropertyOf owl:topDataProperty ;
           rdfs:domain :Card ;
           rdfs:comment "Media item data for a audio, an image or other types of media."@en ;
           rdfs:label "media"@en .


###  http://ns.peterkrantz.se/flashcards/2018#relatedWork
:relatedWork rdf:type owl:DatatypeProperty ;
             rdfs:subPropertyOf owl:topDataProperty ;
             rdfs:domain :Stack ;
             rdfs:comment "A related creative work as e.g. a book, a book chapter, a movie or song. This property can be used to connect a stack of cards to a vocabulary from a chapter in a language textbook."@en ;
             rdfs:label "related work"@en .


###  http://ns.peterkrantz.se/flashcards/2018#sortOrder
:sortOrder rdf:type owl:DatatypeProperty ;
           rdfs:domain :Card ;
           rdfs:range xsd:positiveInteger ;
           rdfs:comment "The initial card sort order expressed as an integer value. The sort order should be used as a suggestion, e.g. when no other sort order exists, and may be ignored by users and tools."@en ;
           rdfs:label "sort order"@en .


###  http://ns.peterkrantz.se/flashcards/2018#text
:text rdf:type owl:DatatypeProperty ;
      rdfs:domain :Card ;
      rdfs:comment "Text content for this object."@en ;
      rdfs:label "text"@en .


#################################################################
#    Classes
#################################################################

###  http://ns.peterkrantz.se/flashcards/2018#Answer
:Answer rdf:type owl:Class ;
        <http://purl.org/dc/terms/isPartOf> :Card ;
        rdfs:comment "An answer to a related test."@en ;
        rdfs:label "Answer"@en .


###  http://ns.peterkrantz.se/flashcards/2018#Card
:Card rdf:type owl:Class ;
      <http://purl.org/dc/terms/isPartOf> :Stack ;
      rdfs:comment "A physical or virtual card bearing information such as words, images or numbers, on either or both sides. Used in classroom drills or in private study. The card has an associated test and an answer."@en ;
      rdfs:label "Card"@en .


###  http://ns.peterkrantz.se/flashcards/2018#Stack
:Stack rdf:type owl:Class ;
       <http://purl.org/dc/terms/hasPart> :Card ;
       rdfs:comment "A stack represents a collection of cards and is typically used to group cards belonging to a topic being studied. E.g. a collection of cards containing vocabulary for a chapter in a language textbook."@en ;
       rdfs:label "Stack"@en .


###  http://ns.peterkrantz.se/flashcards/2018#Test
:Test rdf:type owl:Class ;
      <http://purl.org/dc/terms/isPartOf> :Card ;
      rdfs:comment "The information the user is trying to memorize. Representing the front side of a physical card."@en ;
      rdfs:label "Test"@en .


#################################################################
#    General axioms
#################################################################

[ rdf:type owl:AllDisjointClasses ;
  owl:members ( :Answer
                :Card
                :Stack
                :Test
              )
] .


###  Generated by the OWL API (version 5.1.7) https://github.com/owlcs/owlapi/
